Add nesting support lemmas

matching-logic/src/SyntacticConstruct.v
@@ -27,40 +27,44 @@ Section with_signature.
    and has to have certain properties about well-formedness
    and substitution.
 *)
-Class EBinder (ebinder : Pattern -> Pattern)
-    (fevo: db_index -> Pattern -> Pattern -> Pattern)
-    (fsvo: db_index -> Pattern -> Pattern -> Pattern)
+Class (* E *) Binder (ebinder : Pattern -> Pattern)
+    (bevo: db_index -> Pattern -> Pattern -> Pattern)
+    (bsvo: db_index -> Pattern -> Pattern -> Pattern)
+    (fevo: evar -> Pattern -> Pattern -> Pattern)
+    (fsvo: svar -> Pattern -> Pattern -> Pattern)
     (feq: evar -> db_index -> Pattern -> Pattern)
     (fsq: svar -> db_index -> Pattern -> Pattern)
     :=
 {
-ebinder_bevar_subst :
+binder_bevar_subst :
   forall ψ,
     well_formed_closed ψ ->
     forall n ϕ,
-      bevar_subst (ebinder ϕ) ψ n = fevo n ψ ϕ ;
-ebinder_bsvar_subst :
+      bevar_subst (ebinder ϕ) ψ n = bevo n ψ ϕ ;
+binder_bsvar_subst :
   forall ψ,
     well_formed_closed ψ ->
     forall n ϕ,
-      bsvar_subst (ebinder ϕ) ψ n = fsvo n ψ ϕ ;
-ebinder_free_evar_subst :
+      bsvar_subst (ebinder ϕ) ψ n = bsvo n ψ ϕ ;
+binder_free_evar_subst :
   forall ψ x φ,
-    (ebinder φ).[[evar: x ↦ ψ]] = ebinder (φ.[[evar: x ↦ ψ]]);
-ebinder_free_svar_subst :
+    (ebinder φ).[[evar: x ↦ ψ]] = fevo x ψ φ;
+binder_free_svar_subst :
   forall ψ x φ,
-    (ebinder φ).[[svar: x ↦ ψ]] = ebinder (φ.[[svar: x ↦ ψ]]);
-ebinder_evar_quantify :
+    (ebinder φ).[[svar: x ↦ ψ]] = fsvo x ψ φ;
+binder_evar_quantify :
   forall n x φ,
     evar_quantify x n (ebinder φ) = feq x n φ;
-ebinder_svar_quantify :
+binder_svar_quantify :
   forall n x φ,
     svar_quantify x n (ebinder φ) = fsq x n φ;
 }.
 
-Class SBinder (sbinder : Pattern -> Pattern)
-    (fevo: db_index -> Pattern -> Pattern -> Pattern)
-    (fsvo: db_index -> Pattern -> Pattern -> Pattern)
+(* Class SBinder (sbinder : Pattern -> Pattern)
+    (bevo: db_index -> Pattern -> Pattern -> Pattern)
+    (bsvo: db_index -> Pattern -> Pattern -> Pattern)
+    (fevo: evar -> Pattern -> Pattern -> Pattern)
+    (fsvo: svar -> Pattern -> Pattern -> Pattern)
     (feq: evar -> db_index -> Pattern -> Pattern)
     (fsq: svar -> db_index -> Pattern -> Pattern)
 :=
@@ -69,25 +73,25 @@ sbinder_bevar_subst :
   forall ψ,
     well_formed_closed ψ ->
     forall n φ,
-      bevar_subst (sbinder φ) ψ n = fevo n ψ φ ;
+      bevar_subst (sbinder φ) ψ n = bevo n ψ φ ;
 sbinder_bsvar_subst :
   forall ψ,
     well_formed_closed ψ ->
     forall n φ,
-      bsvar_subst (sbinder φ) ψ n = fsvo n ψ φ ;
+      bsvar_subst (sbinder φ) ψ n = bsvo n ψ φ ;
 sbinder_free_evar_subst :
   forall ψ x φ,
-    (sbinder φ).[[evar: x ↦ ψ]] = sbinder (φ.[[evar: x ↦ ψ]]);
+    (sbinder φ).[[evar: x ↦ ψ]] = fevo x ψ φ;
 sbinder_free_svar_subst :
   forall ψ x φ,
-    (sbinder φ).[[svar: x ↦ ψ]] = sbinder (φ.[[svar: x ↦ ψ]]);
+    (sbinder φ).[[svar: x ↦ ψ]] = fsvo x ψ φ;
 sbinder_evar_quantify :
   forall n x φ,
     evar_quantify x n (sbinder φ) = feq x n φ;
 sbinder_svar_quantify :
   forall n x φ,
     svar_quantify x n (sbinder φ) = fsq x n φ;
-}.
+}. *)
 
 (* Non-variable nullary operation *)
 Class NVNullary (nvnullary : Pattern) :=
@@ -175,85 +179,85 @@ binary_wf : forall ψ1 ψ2, well_formed ψ1 -> well_formed ψ2 -> well_formed (b
 }.
 
 Definition simpl_bevar_subst' :=
-(@ebinder_bevar_subst,
- @sbinder_bevar_subst,
+(@binder_bevar_subst,
+ (* @sbinder_bevar_subst, *)
  @nvnullary_bevar_subst,
  @unary_bevar_subst,
  @binary_bevar_subst
 ).
 
 Definition simpl_bsvar_subst' :=
-(@ebinder_bsvar_subst,
- @sbinder_bsvar_subst,
+(@binder_bsvar_subst,
+ (* @sbinder_bsvar_subst, *)
  @nvnullary_bsvar_subst,
  @unary_bsvar_subst,
  @binary_bsvar_subst
 ).
 
 Definition simpl_free_evar_subst' :=
-(@ebinder_free_evar_subst,
- @sbinder_free_evar_subst,
+(@binder_free_evar_subst,
+(*  @sbinder_free_evar_subst, *)
  @nvnullary_free_evar_subst,
  @unary_free_evar_subst,
  @binary_free_evar_subst
 ).
 
 Definition simpl_free_svar_subst' :=
-(@ebinder_free_svar_subst,
- @sbinder_free_svar_subst,
+(@binder_free_svar_subst,
+(*  @sbinder_free_svar_subst, *)
  @nvnullary_free_svar_subst,
  @unary_free_svar_subst,
  @binary_free_svar_subst
 ).
 
 Definition simpl_evar_quantify' :=
-(@ebinder_evar_quantify,
- @sbinder_evar_quantify,
+(@binder_evar_quantify,
+(*  @sbinder_evar_quantify, *)
  @nvnullary_evar_quantify,
  @unary_evar_quantify,
  @binary_evar_quantify
 ).
 
 Definition simpl_svar_quantify' :=
-(@ebinder_svar_quantify,
- @sbinder_svar_quantify,
+(@binder_svar_quantify,
+(*  @sbinder_svar_quantify, *)
  @nvnullary_svar_quantify,
  @unary_svar_quantify,
  @binary_svar_quantify
 ).
 
 #[global]
-Instance EBinder_exists : EBinder patt_exists _ _ _ _ :=
+Instance Binder_exists : Binder patt_exists _ _ _ _ _ _ :=
 {|
-ebinder_bevar_subst := bevar_subst_exists ;
-ebinder_bsvar_subst := bsvar_subst_exists ;
-ebinder_free_evar_subst := free_evar_subst_exists;
-ebinder_free_svar_subst := free_svar_subst_exists;
-ebinder_evar_quantify := evar_quantify_exists;
-ebinder_svar_quantify := svar_quantify_exists;
+binder_bevar_subst := bevar_subst_exists ;
+binder_bsvar_subst := bsvar_subst_exists ;
+binder_free_evar_subst := free_evar_subst_exists;
+binder_free_svar_subst := free_svar_subst_exists;
+binder_evar_quantify := evar_quantify_exists;
+binder_svar_quantify := svar_quantify_exists;
 |}.
 
 #[global]
-Instance SBinder_mu : SBinder patt_mu _ _ _ _ :=
+Instance Binder_mu : Binder patt_mu _ _ _ _ _ _ :=
 {|
-sbinder_bevar_subst := bevar_subst_mu ;
-sbinder_bsvar_subst := bsvar_subst_mu ;
-sbinder_free_evar_subst := free_evar_subst_mu;
-sbinder_free_svar_subst := free_svar_subst_mu;
-sbinder_evar_quantify := evar_quantify_mu;
-sbinder_svar_quantify := svar_quantify_mu;
+binder_bevar_subst := bevar_subst_mu ;
+binder_bsvar_subst := bsvar_subst_mu ;
+binder_free_evar_subst := free_evar_subst_mu;
+binder_free_svar_subst := free_svar_subst_mu;
+binder_evar_quantify := evar_quantify_mu;
+binder_svar_quantify := svar_quantify_mu;
 |}.
 
 
 #[global]
-Program Instance NVNullary_bott : NVNullary patt_bott :=
+Instance NVNullary_bott : NVNullary patt_bott :=
 {|
 nvnullary_bevar_subst := bevar_subst_bott ;
 nvnullary_bsvar_subst := bsvar_subst_bott ;
-nvnullary_free_evar_subst := free_evar_subst_bott;
-nvnullary_free_svar_subst := free_svar_subst_bott;
-nvnullary_evar_quantify := evar_quantify_bott;
-nvnullary_svar_quantify := svar_quantify_bott;
+nvnullary_free_evar_subst := ltac:(reflexivity);
+nvnullary_free_svar_subst := ltac:(reflexivity);
+nvnullary_evar_quantify := ltac:(reflexivity);
+nvnullary_svar_quantify := ltac:(reflexivity);
 nvnullary_wf := well_formed_bott ;
 |}.
 
@@ -262,10 +266,10 @@ Instance NVNullary_sym s : NVNullary (patt_sym s) :=
 {|
 nvnullary_bevar_subst := λ ψ (wfcψ : well_formed_closed ψ) n, @bevar_subst_sym Σ ψ wfcψ n s ;
 nvnullary_bsvar_subst := λ ψ (wfcψ : well_formed_closed ψ) n, @bsvar_subst_sym Σ ψ wfcψ n s;
-nvnullary_free_evar_subst := λ ψ x, @free_evar_subst_sym Σ ψ x s;
-nvnullary_free_svar_subst := λ ψ x, @free_svar_subst_sym Σ ψ x s;
-nvnullary_evar_quantify := λ ψ x, @evar_quantify_sym Σ ψ x s;
-nvnullary_svar_quantify := λ ψ x, @svar_quantify_sym Σ ψ x s;
+nvnullary_free_evar_subst := ltac:(reflexivity);
+nvnullary_free_svar_subst := ltac:(reflexivity);
+nvnullary_evar_quantify := ltac:(reflexivity);
+nvnullary_svar_quantify := ltac:(reflexivity);
 nvnullary_wf := (well_formed_sym s) ;
 |}.
 
@@ -274,10 +278,10 @@ Instance Binary_app : Binary patt_app :=
 {|
 binary_bevar_subst := bevar_subst_app ;
 binary_bsvar_subst := bsvar_subst_app ;
-binary_free_evar_subst := free_evar_subst_app;
-binary_free_svar_subst := free_svar_subst_app;
-binary_evar_quantify := evar_quantify_app;
-binary_svar_quantify := svar_quantify_app;
+binary_free_evar_subst := ltac:(reflexivity);
+binary_free_svar_subst := ltac:(reflexivity);
+binary_evar_quantify := ltac:(reflexivity);
+binary_svar_quantify := ltac:(reflexivity);
 binary_wf := well_formed_app ;
 |}.
 
@@ -286,10 +290,10 @@ Instance Binary_imp : Binary patt_imp :=
 {|
 binary_bevar_subst := bevar_subst_imp ;
 binary_bsvar_subst := bsvar_subst_imp ;
-binary_free_evar_subst := free_evar_subst_imp;
-binary_free_svar_subst := free_svar_subst_imp;
-binary_evar_quantify := evar_quantify_imp;
-binary_svar_quantify := svar_quantify_imp;
+binary_free_evar_subst := ltac:(reflexivity);
+binary_free_svar_subst := ltac:(reflexivity);
+binary_evar_quantify := ltac:(reflexivity);
+binary_svar_quantify := ltac:(reflexivity);
 binary_wf := well_formed_imp ;
 |}.
 
