matching-logic/src/Theories/Definedness_Syntax.v
@@ -176,28 +176,16 @@ Section definedness.
   Lemma bsvar_subst_defined ψ (wfcψ : well_formed_closed ψ) x ϕ :
     bsvar_subst (patt_defined ϕ) ψ x = patt_defined (bsvar_subst ϕ ψ x).
   Proof. unfold patt_defined. cbn. auto. Qed.
-  Lemma free_evar_subst_defined ψ x ϕ :
-    free_evar_subst (patt_defined ϕ) ψ x = patt_defined (free_evar_subst ϕ ψ x).
-  Proof. unfold patt_defined. cbn. auto. Qed.
-  Lemma free_svar_subst_defined ψ x ϕ :
-    free_svar_subst (patt_defined ϕ) ψ x = patt_defined (free_svar_subst ϕ ψ x).
-  Proof. unfold patt_defined. cbn. auto. Qed.
-  Lemma evar_quantify_defined x db ϕ :
-    evar_quantify db x (patt_defined ϕ) = patt_defined (evar_quantify db x ϕ).
-  Proof. unfold patt_defined. cbn. auto. Qed.
-  Lemma svar_quantify_defined X Db ϕ :
-    svar_quantify Db X (patt_defined ϕ) = patt_defined (svar_quantify Db X ϕ).
-  Proof. unfold patt_defined. cbn. auto. Qed.
 
   #[global]
    Instance Unary_defined : Unary patt_defined :=
     {| unary_bevar_subst := bevar_subst_defined ;
        unary_bsvar_subst := bsvar_subst_defined ;
        unary_wf := well_formed_defined ;
-       unary_free_evar_subst := free_evar_subst_defined ;
-       unary_free_svar_subst := free_svar_subst_defined ;
-       unary_evar_quantify := evar_quantify_defined ;
-       unary_svar_quantify := svar_quantify_defined ;
+       unary_free_evar_subst := ltac:(reflexivity) ;
+       unary_free_svar_subst := ltac:(reflexivity) ;
+       unary_evar_quantify := ltac:(reflexivity) ;
+       unary_svar_quantify := ltac:(reflexivity) ;
     |}.
   
 
@@ -207,28 +195,16 @@ Section definedness.
   Lemma bsvar_subst_total ψ (wfcψ : well_formed_closed ψ) x ϕ :
     bsvar_subst (patt_total ϕ) ψ x = patt_total (bsvar_subst ϕ ψ x).
   Proof. unfold patt_total. simpl_bsvar_subst. reflexivity. Qed.
-  Lemma free_evar_subst_total ψ x ϕ :
-    free_evar_subst (patt_total ϕ) ψ x = patt_total (free_evar_subst ϕ ψ x).
-  Proof. unfold patt_total. cbn. auto. Qed.
-  Lemma free_svar_subst_total ψ x ϕ :
-    free_svar_subst (patt_total ϕ) ψ x = patt_total (free_svar_subst ϕ ψ x).
-  Proof. unfold patt_total. cbn. auto. Qed.
-  Lemma evar_quantify_total x db ϕ :
-    evar_quantify db x (patt_total ϕ) = patt_total (evar_quantify db x ϕ).
-  Proof. unfold patt_total. cbn. auto. Qed.
-  Lemma svar_quantify_total X Db ϕ :
-    svar_quantify Db X (patt_total ϕ) = patt_total (svar_quantify Db X ϕ).
-  Proof. unfold patt_total. cbn. auto. Qed.
 
   #[global]
    Instance Unary_total : Unary patt_total :=
     {| unary_bevar_subst := bevar_subst_total ;
        unary_bsvar_subst := bsvar_subst_total ;
        unary_wf := well_formed_total ;
-       unary_free_evar_subst := free_evar_subst_total ;
-       unary_free_svar_subst := free_svar_subst_total ;
-       unary_evar_quantify := evar_quantify_total ;
-       unary_svar_quantify := svar_quantify_total ;
+       unary_free_evar_subst := ltac:(reflexivity) ;
+       unary_free_svar_subst := ltac:(reflexivity) ;
+       unary_evar_quantify := ltac:(reflexivity) ;
+       unary_svar_quantify := ltac:(reflexivity) ;
     |}.
 
 
@@ -238,28 +214,16 @@ Section definedness.
   Lemma bsvar_subst_equal ψ (wfcψ : well_formed_closed ψ) x ϕ₁ ϕ₂ :
     bsvar_subst (patt_equal ϕ₁ ϕ₂) ψ x = patt_equal (bsvar_subst ϕ₁ ψ x) (bsvar_subst ϕ₂ ψ x).
   Proof. unfold patt_equal. simpl_bsvar_subst. reflexivity. Qed.
-  Lemma free_evar_subst_equal ψ x ϕ₁ ϕ₂ :
-    free_evar_subst (patt_equal ϕ₁ ϕ₂) ψ x = patt_equal (free_evar_subst ϕ₁ ψ x) (free_evar_subst ϕ₂ ψ x).
-  Proof. unfold patt_equal. cbn. auto. Qed.
-  Lemma free_svar_subst_equal ψ x ϕ₁ ϕ₂:
-    free_svar_subst (patt_equal ϕ₁ ϕ₂) ψ x = patt_equal (free_svar_subst ϕ₁ ψ x) (free_svar_subst ϕ₂ ψ x).
-  Proof. unfold patt_equal. cbn. auto. Qed.
-  Lemma evar_quantify_equal x db ϕ₁ ϕ₂ :
-    evar_quantify db x (patt_equal ϕ₁ ϕ₂) = patt_equal (evar_quantify db x ϕ₁) (evar_quantify db x ϕ₂).
-  Proof. unfold patt_equal. cbn. auto. Qed.
-  Lemma svar_quantify_equal X Db ϕ₁ ϕ₂:
-    svar_quantify Db X (patt_equal ϕ₁ ϕ₂) = patt_equal (svar_quantify Db X ϕ₁) (svar_quantify Db X ϕ₂).
-  Proof. unfold patt_equal. cbn. auto. Qed.
 
   #[global]
    Instance Binary_equal : Binary patt_equal :=
     {| binary_bevar_subst := bevar_subst_equal ;
        binary_bsvar_subst := bsvar_subst_equal ;
        binary_wf := well_formed_equal ;
-       binary_free_evar_subst := free_evar_subst_equal ;
-       binary_free_svar_subst := free_svar_subst_equal ;
-       binary_evar_quantify := evar_quantify_equal ;
-       binary_svar_quantify := svar_quantify_equal ;
+       binary_free_evar_subst := ltac:(reflexivity) ;
+       binary_free_svar_subst := ltac:(reflexivity) ;
+       binary_evar_quantify := ltac:(reflexivity) ;
+       binary_svar_quantify := ltac:(reflexivity) ;
     |}.
   
   Lemma bevar_subst_subseteq ψ (wfcψ : well_formed_closed ψ) x ϕ₁ ϕ₂ :
@@ -268,28 +232,16 @@ Section definedness.
   Lemma bsvar_subst_subseteq ψ (wfcψ : well_formed_closed ψ) x ϕ₁ ϕ₂ :
     bsvar_subst (patt_subseteq ϕ₁ ϕ₂) ψ x = patt_subseteq (bsvar_subst ϕ₁ ψ x) (bsvar_subst ϕ₂ ψ x).
   Proof. unfold patt_subseteq. simpl_bsvar_subst. reflexivity. Qed.
-  Lemma free_evar_subst_subseteq ψ x ϕ₁ ϕ₂ :
-    free_evar_subst (patt_subseteq ϕ₁ ϕ₂) ψ x = patt_subseteq (free_evar_subst ϕ₁ ψ x) (free_evar_subst ϕ₂ ψ x).
-  Proof. unfold patt_subseteq. cbn. auto. Qed.
-  Lemma free_svar_subst_subseteq ψ x ϕ₁ ϕ₂:
-    free_svar_subst (patt_subseteq ϕ₁ ϕ₂) ψ x = patt_subseteq (free_svar_subst ϕ₁ ψ x) (free_svar_subst ϕ₂ ψ x).
-  Proof. unfold patt_subseteq. cbn. auto. Qed.
-  Lemma evar_quantify_subseteq x db ϕ₁ ϕ₂ :
-    evar_quantify db x (patt_subseteq ϕ₁ ϕ₂) = patt_subseteq (evar_quantify db x ϕ₁) (evar_quantify db x ϕ₂).
-  Proof. unfold patt_subseteq. cbn. auto. Qed.
-  Lemma svar_quantify_subseteq X Db ϕ₁ ϕ₂:
-    svar_quantify Db X (patt_subseteq ϕ₁ ϕ₂) = patt_subseteq (svar_quantify Db X ϕ₁) (svar_quantify Db X ϕ₂).
-  Proof. unfold patt_subseteq. cbn. auto. Qed.
 
   #[global]
    Instance Binary_subseteq : Binary patt_subseteq :=
     {| binary_bevar_subst := bevar_subst_subseteq ;
        binary_bsvar_subst := bsvar_subst_subseteq ;
        binary_wf := well_formed_subseteq ;
-       binary_free_evar_subst := free_evar_subst_subseteq ;
-       binary_free_svar_subst := free_svar_subst_subseteq ;
-       binary_evar_quantify := evar_quantify_subseteq ;
-       binary_svar_quantify := svar_quantify_subseteq ;
+       binary_free_evar_subst := ltac:(reflexivity) ;
+       binary_free_svar_subst := ltac:(reflexivity) ;
+       binary_evar_quantify := ltac:(reflexivity) ;
+       binary_svar_quantify := ltac:(reflexivity) ;
     |}.
 
   Lemma bevar_subst_in ψ (wfcψ : well_formed_closed ψ) x ϕ₁ ϕ₂ :
@@ -298,28 +250,16 @@ Section definedness.
   Lemma bsvar_subst_in ψ (wfcψ : well_formed_closed ψ) x ϕ₁ ϕ₂ :
     bsvar_subst (patt_in ϕ₁ ϕ₂) ψ x = patt_in (bsvar_subst ϕ₁ ψ x) (bsvar_subst ϕ₂ ψ x).
   Proof. unfold patt_in. simpl_bsvar_subst. reflexivity. Qed.
-  Lemma free_evar_subst_in ψ x ϕ₁ ϕ₂ :
-    free_evar_subst (patt_in ϕ₁ ϕ₂) ψ x = patt_in (free_evar_subst ϕ₁ ψ x) (free_evar_subst ϕ₂ ψ x).
-  Proof. unfold patt_in. cbn. auto. Qed.
-  Lemma free_svar_subst_in ψ x ϕ₁ ϕ₂:
-    free_svar_subst (patt_in ϕ₁ ϕ₂) ψ x = patt_in (free_svar_subst ϕ₁ ψ x) (free_svar_subst ϕ₂ ψ x).
-  Proof. unfold patt_in. cbn. auto. Qed.
-  Lemma evar_quantify_in x db ϕ₁ ϕ₂ :
-    evar_quantify db x (patt_in ϕ₁ ϕ₂) = patt_in (evar_quantify db x ϕ₁) (evar_quantify db x ϕ₂).
-  Proof. unfold patt_in. cbn. auto. Qed.
-  Lemma svar_quantify_in X Db ϕ₁ ϕ₂:
-    svar_quantify Db X (patt_in ϕ₁ ϕ₂) = patt_in (svar_quantify Db X ϕ₁) (svar_quantify Db X ϕ₂).
-  Proof. unfold patt_in. cbn. auto. Qed.
 
   #[global]
    Instance Binary_in : Binary patt_in :=
     {| binary_bevar_subst := bevar_subst_in ;
        binary_bsvar_subst := bsvar_subst_in ;
        binary_wf := well_formed_in ;
-       binary_free_evar_subst := free_evar_subst_in ;
-       binary_free_svar_subst := free_svar_subst_in ;
-       binary_evar_quantify := evar_quantify_in ;
-       binary_svar_quantify := svar_quantify_in ;
+       binary_free_evar_subst := ltac:(reflexivity) ;
+       binary_free_svar_subst := ltac:(reflexivity) ;
+       binary_evar_quantify := ltac:(reflexivity) ;
+       binary_svar_quantify := ltac:(reflexivity) ;
     |}.
 
   (* Defines ϕ₁ to be an inversion of ϕ₂ *)
